Improvements from agent review

rocq-skylabs-brick/tests/resolve_template_alias.v
@@ -1,5 +1,6 @@
 Require Import skylabs.prelude.base.
 Require Import skylabs.lang.cpp.syntax.
+Require Import skylabs.lang.cpp.syntax.templates.
 Require Import skylabs.lang.cpp.syntax.dealias.
 Require Import skylabs.lang.cpp.parser.
 Require Import skylabs.lang.cpp.parser.plugin.cpp2v.
@@ -19,6 +20,45 @@ struct DefaultedChain {
   V third;
 };
 
+template <typename T, typename U = bool>
+struct ConcreteDefault {
+  T first;
+  U second;
+};
+
+template <typename T, typename U = T, typename V = U *>
+struct PointerChain {
+  T first;
+  U second;
+  V third;
+};
+
+template <typename T, int N = 0>
+struct ValueDefault {
+  T value;
+};
+
+template <typename T>
+struct TemplateTemplateDefaultArg {
+  T value;
+};
+
+template <template <typename> class TT = TemplateTemplateDefaultArg>
+struct TemplateTemplateDefault {
+};
+
+template <int N>
+struct ValueOuter {
+  template <typename T, typename U = T>
+  struct Inner {
+    T first;
+    U second;
+  };
+};
+
+template <typename T, typename U = T>
+struct ForwardDefault;
+
 template <typename T, typename U = T>
 union DefaultedUnion {
   T first;
@@ -30,6 +70,15 @@ using DefaultedTypeAlias = DefaultedPair<T, U>;
 
 template <typename T, typename U = bool>
 using ExplicitAlias = DefaultedPair<U, T>;
+
+template <typename OuterT>
+struct Outer {
+  template <typename InnerT, typename InnerU = OuterT>
+  struct Inner {
+    InnerT first;
+    InnerU second;
+  };
+};
 
 namespace DefaultNS {
   template <typename T, typename U = T>
@@ -43,6 +92,78 @@ namespace DefaultNS {
 Notation RESOLVE_TYPE input output :=
   (trace.runO (dealias.resolveTN source input%cpp_name) = Some output%cpp_type)
   (only parsing).
+
+Definition lookup_alias_template (n : name) : option (template type) :=
+  translation_unit.maliases source !! n.
+
+Definition alias_template_params (n : name) : option (list temp_param) :=
+  match lookup_alias_template n with
+  | Some t => Some t.(template_params)
+  | None => None
+  end.
+
+Definition alias_template_value (n : name) : option type :=
+  match lookup_alias_template n with
+  | Some t => Some t.(template_value)
+  | None => None
+  end.
+
+Definition template_template_default_alias_name : name :=
+  Ninst (Nglobal (Nid "TemplateTemplateDefault")) [].
+
+Example defaulted_pair_generated_alias_params :
+  alias_template_params "DefaultedPair<$T>"%cpp_name = Some [Ptype "T"].
+Proof. vm_compute. reflexivity. Qed.
+
+Example defaulted_pair_generated_alias_target :
+  alias_template_value "DefaultedPair<$T>"%cpp_name =
+  Some "DefaultedPair<$T, $T>"%cpp_type.
+Proof. vm_compute. reflexivity. Qed.
+
+Example defaulted_pair_does_not_generate_full_arity_alias :
+  lookup_alias_template "DefaultedPair<$T, $U>"%cpp_name = None.
+Proof. vm_compute. reflexivity. Qed.
+
+Example defaulted_chain_one_arg_generated_alias_params :
+  alias_template_params "DefaultedChain<$T>"%cpp_name = Some [Ptype "T"].
+Proof. vm_compute. reflexivity. Qed.
+
+Example defaulted_chain_one_arg_generated_alias_target :
+  alias_template_value "DefaultedChain<$T>"%cpp_name =
+  Some "DefaultedChain<$T, $T, $T>"%cpp_type.
+Proof. vm_compute. reflexivity. Qed.
+
+Example defaulted_chain_two_arg_generated_alias_params :
+  alias_template_params "DefaultedChain<$T, $U>"%cpp_name =
+  Some [Ptype "T"; Ptype "U"].
+Proof. vm_compute. reflexivity. Qed.
+
+Example defaulted_chain_two_arg_generated_alias_target :
+  alias_template_value "DefaultedChain<$T, $U>"%cpp_name =
+  Some "DefaultedChain<$T, $U, $U>"%cpp_type.
+Proof. vm_compute. reflexivity. Qed.
+
+Example concrete_default_generated_alias_target :
+  alias_template_value "ConcreteDefault<$T>"%cpp_name =
+  Some "ConcreteDefault<$T, bool>"%cpp_type.
+Proof. vm_compute. reflexivity. Qed.
+
+Example pointer_chain_generated_alias_target_substitutes_inside_pointer :
+  alias_template_value "PointerChain<$T>"%cpp_name =
+  Some "PointerChain<$T, $T, $T*>"%cpp_type.
+Proof. vm_compute. reflexivity. Qed.
+
+Example value_default_does_not_generate_unsupported_alias :
+  lookup_alias_template "ValueDefault<$T>"%cpp_name = None.
+Proof. vm_compute. reflexivity. Qed.
+
+Example template_template_default_does_not_generate_unsupported_alias :
+  lookup_alias_template template_template_default_alias_name = None.
+Proof. vm_compute. reflexivity. Qed.
+
+Example value_outer_inner_does_not_generate_unsupported_enclosing_alias :
+  lookup_alias_template "ValueOuter<`N>::Inner<$T>"%cpp_name = None.
+Proof. vm_compute. reflexivity. Qed.
 
 Example defaulted_pair_resolves_through_generated_alias :
   RESOLVE_TYPE "DefaultedPair<int>" "DefaultedPair<int, int>".
@@ -70,6 +191,26 @@ Proof. vm_compute. reflexivity. Qed.
 
 Example defaulted_chain_two_arg_template_type_resolves_through_generated_alias :
   RESOLVE_TYPE "DefaultedChain<$T, $U>" "DefaultedChain<$T, $U, $U>".
+Proof. vm_compute. reflexivity. Qed.
+
+Example concrete_default_resolves_through_generated_alias :
+  RESOLVE_TYPE "ConcreteDefault<int>" "ConcreteDefault<int, bool>".
+Proof. vm_compute. reflexivity. Qed.
+
+Example concrete_default_template_type_resolves_through_generated_alias :
+  RESOLVE_TYPE "ConcreteDefault<$T>" "ConcreteDefault<$T, bool>".
+Proof. vm_compute. reflexivity. Qed.
+
+Example pointer_chain_resolves_compound_default_substitution :
+  RESOLVE_TYPE "PointerChain<int>" "PointerChain<int, int, int*>".
+Proof. vm_compute. reflexivity. Qed.
+
+Example pointer_chain_template_type_resolves_compound_default_substitution :
+  RESOLVE_TYPE "PointerChain<$T>" "PointerChain<$T, $T, $T*>".
+Proof. vm_compute. reflexivity. Qed.
+
+Example forward_default_resolves_from_declaration :
+  RESOLVE_TYPE "ForwardDefault<int>" "ForwardDefault<int, int>".
 Proof. vm_compute. reflexivity. Qed.
 
 Example defaulted_union_resolves_through_generated_alias :
@@ -100,9 +241,39 @@ Example explicit_alias_template_type_resolves_via_explicit_body :
   RESOLVE_TYPE "ExplicitAlias<$T>" "DefaultedPair<bool, $T>".
 Proof. vm_compute. reflexivity. Qed.
 
+Example explicit_alias_generated_alias_target_preserves_explicit_alias :
+  alias_template_value "ExplicitAlias<$T>"%cpp_name =
+  Some "ExplicitAlias<$T, bool>"%cpp_type.
+Proof. vm_compute. reflexivity. Qed.
+
+Example nested_default_generated_alias_params_include_outer_param :
+  alias_template_params "Outer<$OuterT>::Inner<$InnerT>"%cpp_name =
+  Some [Ptype "OuterT"; Ptype "InnerT"].
+Proof. vm_compute. reflexivity. Qed.
+
+Example nested_default_generated_alias_target_uses_outer_param :
+  alias_template_value "Outer<$OuterT>::Inner<$InnerT>"%cpp_name =
+  Some "Outer<$OuterT>::Inner<$InnerT, $OuterT>"%cpp_type.
+Proof. vm_compute. reflexivity. Qed.
+
+Example nested_default_resolves_through_generated_alias :
+  RESOLVE_TYPE "Outer<int>::Inner<bool>"
+               "Outer<int>::Inner<bool, int>".
+Proof. vm_compute. reflexivity. Qed.
+
+Example nested_default_template_type_resolves_through_generated_alias :
+  RESOLVE_TYPE "Outer<$T>::Inner<$U>"
+               "Outer<$T>::Inner<$U, $T>".
+Proof. vm_compute. reflexivity. Qed.
+
 Example scoped_default_resolves_through_generated_alias :
   RESOLVE_TYPE "DefaultNS::ScopedDefault<int>"
                "DefaultNS::ScopedDefault<int, int>".
+Proof. vm_compute. reflexivity. Qed.
+
+Example scoped_default_generated_alias_target :
+  alias_template_value "DefaultNS::ScopedDefault<$T>"%cpp_name =
+  Some "DefaultNS::ScopedDefault<$T, $T>"%cpp_type.
 Proof. vm_compute. reflexivity. Qed.
 
 Example scoped_default_template_type_resolves_through_generated_alias :
